Start improving speed by removing calls to trefl and as many calls to normalizer as possible
The calls to trefl are very expensive and useless. Instead, we admit the
proof (the system needs to be improved to make it more robust and track
errors).
Besides, the calls to the normalizer are very expensive. The problem is
that we use the normalizer a lot for variables substitutions. We thus
implemented our custom substitution functions.

FEM.Process.fst
@@ -14,6 +14,8 @@ open FStar.Mul
 
 #push-options "--z3rlimit 15 --fuel 0 --ifuel 1"
 
+let print_info = print
+
 (* TODO: move to FStar.Tactics.Util.fst *)
 #push-options "--ifuel 1"
 val iteri_aux: int -> (int -> 'a -> Tac unit) -> list 'a -> Tac unit
@@ -123,7 +125,11 @@ let rec filter_ascriptions t =
 /// before exporting, because we may have inserted ascriptions on purpose, which
 /// would then be filtered away.
 val prettify_term : term -> Tac term
-let prettify_term t = filter_ascriptions t
+let prettify_term t =
+  print_info "start prettify";
+  let t' = filter_ascriptions t in
+  print_info "end prettify";
+  t'
 
 (*** General utilities *)
 // TODO: use more
@@ -357,14 +363,148 @@ let genv_push_fresh_bv (ge : genv) (basename : string) (ty : typ) : Tac (genv & 
   let ge', b = genv_push_fresh_binder ge basename ty in
   ge', bv_of_binder b
 
+// TODO: this function is super slow because normalization is very expensive
+// -> rewrite it
 /// Perform a variable substitution in a term
 val apply_subst : env -> term -> list (bv & term) -> Tac term
-let apply_subst e t subst =
+// Whenever we encounter a construction which introduces a binder, we need to apply
+// the substitution in the binder type. Note that this gives a new binder, with
+// which we need to replace the old one in what follows
+val apply_subst_in_bv : env -> bv -> list (bv & term) -> Tac (bv & list (bv & term))
+val apply_subst_in_binder : env -> binder -> list (bv & term) -> Tac (binder & list (bv & term))
+val apply_subst_in_comp : env -> comp -> list (bv & term) -> Tac comp
+val apply_subst_in_pattern : env -> pattern -> list (bv & term) -> Tac (pattern & list (bv & term))
+(*let apply_subst e t subst =
   let bl, vl = unzip subst in
   let bl = List.Tot.map mk_binder bl in
   let t1 = mk_abs t bl in
   let t2 = mk_e_app t1 vl in
-  norm_term_env e [] t2
+  norm_term_env e [] t2 *)
+
+let rec apply_subst e t subst =
+  match inspect t with
+  | Tv_Var b ->
+    begin match bind_map_get subst b with
+    | None -> t
+    | Some t' -> t'
+    end
+  | Tv_BVar b ->
+    (* Note: Tv_BVar shouldn't happen *)
+    begin match bind_map_get subst b with
+    | None -> t
+    | Some t' -> t'
+    end
+  | Tv_FVar _ -> t
+  | Tv_App hd (a,qual) ->
+    let hd = apply_subst e hd subst in
+    let a = apply_subst e a subst in
+    pack (Tv_App hd (a, qual))
+  | Tv_Abs br body ->
+    let body = apply_subst e body subst in
+    pack (Tv_Abs br body)
+  | Tv_Arrow br c ->
+    let br, subst = apply_subst_in_binder e br subst in
+    let c = apply_subst_in_comp e c subst in
+    pack (Tv_Arrow br c)
+  | Tv_Type () -> t
+  | Tv_Refine bv ref ->
+    let bv, subst = apply_subst_in_bv e bv subst in
+    let ref = apply_subst e ref subst in
+    pack (Tv_Refine bv ref)
+  | Tv_Const _ -> t
+  | Tv_Uvar _ _ -> t
+  | Tv_Let recf attrs bv def body ->
+    (* No need to substitute in the attributes - that we filter for safety *)
+    let bv, subst = apply_subst_in_bv e bv subst in
+    let def = apply_subst e def subst in
+    let body = apply_subst e body subst in
+    pack (Tv_Let recf [] bv def body)
+  | Tv_Match scrutinee branches -> (* TODO: type of pattern variables *)
+    let scrutinee = apply_subst e scrutinee subst in
+    (* For the branches: we don't need to explore the patterns *)
+    let apply_subst_in_branch branch =
+      let pat, tm = branch in
+      let pat, subst = apply_subst_in_pattern e pat subst in
+      let tm = apply_subst e tm subst in
+      pat, tm
+    in
+    let branches = map apply_subst_in_branch branches in
+    pack (Tv_Match scrutinee branches)
+  | Tv_AscribedT exp ty tac ->
+    let exp = apply_subst e exp subst in
+    let ty = apply_subst e ty subst in
+    (* no need to apply it on the tactic - that we filter for safety *)
+    pack (Tv_AscribedT exp ty None)
+  | Tv_AscribedC exp c tac ->
+    let exp = apply_subst e exp subst in
+    let c = apply_subst_in_comp e c subst in
+    (* no need to apply it on the tactic - that we filter for safety *)
+    pack (Tv_AscribedC exp c None)
+  | _ ->
+    (* Unknown *)
+    t
+
+and apply_subst_in_bv e bv subst =
+  let bvv = inspect_bv bv in
+  let ty = apply_subst e bvv.bv_sort subst in
+  let bv' = Tactics.fresh_bv_named bvv.bv_ppname ty in
+  bv', (bv, pack (Tv_Var bv'))::subst
+
+and apply_subst_in_binder e br subst =
+  let bv, qual = inspect_binder br in
+  let bv, subst = apply_subst_in_bv e bv subst in
+  pack_binder bv qual, subst 
+
+and apply_subst_in_comp e c subst =
+  let subst = (fun x -> apply_subst e x subst) in
+  let subst_in_aqualv a : Tac aqualv =
+    match a with
+    | Q_Implicit
+    | Q_Explicit -> a
+    | Q_Meta t -> Q_Meta (subst t)
+    | Q_Meta_attr t -> Q_Meta_attr (subst t)
+  in
+  match inspect_comp c with
+  | C_Total ret decr ->
+    let ret = subst ret in
+    let decr = opt_tapply subst decr in
+    pack_comp (C_Total ret decr)
+  | C_GTotal ret decr ->
+    let ret = subst ret in
+    let decr = opt_tapply subst decr in
+    pack_comp (C_GTotal ret decr)
+  | C_Lemma pre post patterns ->
+    let pre = subst pre in
+    let post = subst post in
+    let patterns = subst patterns in
+    pack_comp (C_Lemma pre post patterns)
+  | C_Eff us eff_name result eff_args ->
+    let result = subst result in
+    let eff_args = map (fun (x, a) -> (subst x, subst_in_aqualv a)) eff_args in
+    pack_comp (C_Eff us eff_name result eff_args)
+
+and apply_subst_in_pattern e pat subst =
+  match pat with
+  | Pat_Constant _ -> pat, subst
+  | Pat_Cons fv patterns ->
+    (* The types of the variables in the patterns should be independent of each
+     * other: we use fold_left only to incrementally update the substitution *)
+    let patterns, subst =
+      fold_right (fun (pat, b) (pats, subst) ->
+                      let pat, subst = apply_subst_in_pattern e pat subst in
+                      ((pat, b) :: pats, subst)) patterns ([], subst)
+    in
+    Pat_Cons fv patterns, subst
+  | Pat_Var bv ->
+    let bv, subst = apply_subst_in_bv e bv subst in
+    Pat_Var bv, subst
+  | Pat_Wild bv ->
+    let bv, subst = apply_subst_in_bv e bv subst in
+    Pat_Wild bv, subst
+  | Pat_Dot_Term bv t ->
+    let bv, subst = apply_subst_in_bv e bv subst in
+    let t = apply_subst e t subst in
+    Pat_Dot_Term bv t, subst
 
 val opt_apply_subst : env -> option term -> list (bv & term) -> Tac (option term)
 let opt_apply_subst e opt_t subst =
@@ -551,36 +691,9 @@ let safe_typ_or_comp dbg e t =
                    "\n-comp: " ^ acomp_to_string c);
     Some (TC_Comp c [])
 
-/// Substitute a binder by a term in a comp
 val subst_bv_in_comp : env -> bv -> term -> comp -> Tac comp
 let subst_bv_in_comp e b t c =
-  let subst = [(b,t)] in
-  let subst = (fun x -> apply_subst e x subst) in
-  let subst_in_aqualv a : Tac aqualv =
-    match a with
-    | Q_Implicit
-    | Q_Explicit -> a
-    | Q_Meta t -> Q_Meta (subst t)
-    | Q_Meta_attr t -> Q_Meta_attr (subst t)
-  in
-  match inspect_comp c with
-  | C_Total ret decr ->
-    let ret = subst ret in
-    let decr = opt_tapply subst decr in
-    pack_comp (C_Total ret decr)
-  | C_GTotal ret decr ->
-    let ret = subst ret in
-    let decr = opt_tapply subst decr in
-    pack_comp (C_GTotal ret decr)
-  | C_Lemma pre post patterns ->
-    let pre = subst pre in
-    let post = subst post in
-    let patterns = subst patterns in
-    pack_comp (C_Lemma pre post patterns)
-  | C_Eff us eff_name result eff_args ->
-    let result = subst result in
-    let eff_args = map (fun (x, a) -> (subst x, subst_in_aqualv a)) eff_args in
-    pack_comp (C_Eff us eff_name result eff_args)
+  apply_subst_in_comp e c [(b, t)]
 
 val subst_binder_in_comp : env -> binder -> term -> comp -> Tac comp
 let subst_binder_in_comp e b t c =
@@ -589,50 +702,54 @@ let subst_binder_in_comp e b t c =
 /// Utility for computations: unfold a type until it is of the form Tv_Arrow _ _,
 /// fail otherwise
 val unfold_until_arrow : env -> typ -> Tac typ
-let rec unfold_until_arrow e ty =
-  (* Start by normalizing the term *)
-  let ty = norm_term_env e [] ty in
-  (* Helper to unfold top-level identifiers *)
-  let unfold_fv (fv : fv) : Tac term =
-    let ty = pack (Tv_FVar fv) in
-    let fvn = flatten_name (inspect_fv fv) in
-    (* unfold the top level binding, check that it has changed, and recurse *)
-    let ty' = norm_term_env e [delta_only [fvn]] ty in
-    (* I'm not confident about using eq_term here *)
-    begin match inspect ty' with
-    | Tv_FVar fv' ->
-      if flatten_name (inspect_fv fv') = fvn
-      then mfail ("unfold_until_arrow: could not unfold: " ^ term_to_string ty) else ty'
-    | _ -> ty'
-    end
-  in
-  (* Inspect *)
-  match inspect ty with
-  | Tv_Arrow _ _ -> ty
-  | Tv_FVar fv ->
-    (* Try to unfold the top-level identifier and recurse *)
-    let ty' = unfold_fv fv in
-    unfold_until_arrow e ty'
-  | Tv_App _ _ ->
-    (* Strip all the parameters, try to unfold the head and recurse *)
-    let hd, args = collect_app ty in
-    begin match inspect hd with
+let rec unfold_until_arrow e ty0 =
+  if Tv_Arrow? (inspect ty0) then ty0
+  else
+    begin
+    (* Start by normalizing the term - note that this operation is expensive *)
+    let ty = norm_term_env e [] ty0 in
+    (* Helper to unfold top-level identifiers *)
+    let unfold_fv (fv : fv) : Tac term =
+      let ty = pack (Tv_FVar fv) in
+      let fvn = flatten_name (inspect_fv fv) in
+      (* unfold the top level binding, check that it has changed, and recurse *)
+      let ty' = norm_term_env e [delta_only [fvn]] ty in
+      (* I'm not confident about using eq_term here *)
+      begin match inspect ty' with
+      | Tv_FVar fv' ->
+        if flatten_name (inspect_fv fv') = fvn
+        then mfail ("unfold_until_arrow: could not unfold: " ^ term_to_string ty0) else ty'
+      | _ -> ty'
+      end
+    in
+    (* Inspect *)
+    match inspect ty with
+    | Tv_Arrow _ _ -> ty
     | Tv_FVar fv ->
-      let hd' = unfold_fv fv in
-      let ty' = mk_app hd' args in
+      (* Try to unfold the top-level identifier and recurse *)
+      let ty' = unfold_fv fv in
       unfold_until_arrow e ty'
-    | _ -> mfail ("unfold_until_arrow: could not unfold: " ^ term_to_string ty)
+    | Tv_App _ _ ->
+      (* Strip all the parameters, try to unfold the head and recurse *)
+      let hd, args = collect_app ty in
+      begin match inspect hd with
+      | Tv_FVar fv ->
+        let hd' = unfold_fv fv in
+        let ty' = mk_app hd' args in
+        unfold_until_arrow e ty'
+      | _ -> mfail ("unfold_until_arrow: could not unfold: " ^ term_to_string ty0)
+      end
+    | Tv_Refine bv ref ->
+      (* Continue with the type of bv *)
+      let ty' = type_of_bv bv in
+      unfold_until_arrow e ty'
+    | Tv_AscribedT body _ _
+    | Tv_AscribedC body _ _ ->
+      unfold_until_arrow e body
+    | _ ->
+      (* Other situations: don't know what to do *)
+      mfail ("unfold_until_arrow: could not unfold: " ^ term_to_string ty0)
     end
-  | Tv_Refine bv ref ->
-    (* Continue with the type of bv *)
-    let ty' = type_of_bv bv in
-    unfold_until_arrow e ty'
-  | Tv_AscribedT body _ _
-  | Tv_AscribedC body _ _ ->
-    unfold_until_arrow e body
-  | _ ->
-    (* Other situations: don't know what to do *)
-    mfail ("unfold_until_arrow: could not unfold: " ^ term_to_string ty)
 
 /// Instantiate a comp
 val inst_comp_once : env -> comp -> term -> Tac comp
@@ -668,10 +785,15 @@ let _abs_update_typ (b:binder) (ty:typ) (pl:list binder) (e:env) :
   Tac typ_or_comp =
   (* Try to reveal an arrow *)
   try
+    print_info "starting unfold_until_arrow";
+//    print_info ("_abs_update_typ: " ^ term_to_string ty);
     let ty' = unfold_until_arrow e ty in
+    print_info "ended unfold_until_arrow";
     begin match inspect ty' with
     | Tv_Arrow b1 c1 ->
+      print_info "starting subst_binder_in_comp";
       let c1' = subst_binder_in_comp e b1 (pack (Tv_Var (bv_of_binder b))) c1 in
+      print_info "ended subst_binder_in_comp";
       TC_Comp c1' (b :: pl)
     | _ -> (* Inconsistent state *)
       mfail "_abs_update_typ: inconsistent state"
@@ -688,7 +810,9 @@ let abs_update_typ_or_comp (b:binder) (c : typ_or_comp) (e:env) : Tac typ_or_com
     (* Note that the computation is not necessarily pure, in which case we might
      * want to do something with the effect arguments (pre, post...) - for
      * now we just ignore them *)
+    print_info "starting get_comp_ret_type";
     let ty = get_comp_ret_type v in
+    print_info "starting _apt_update_typ";
     _abs_update_typ b ty pl e
 
 val abs_update_opt_typ_or_comp : binder -> option typ_or_comp -> env ->
@@ -761,6 +885,7 @@ val explore_pattern :
 
 (* TODO: carry around the list of encompassing terms *)
 let rec explore_term dbg dfs #a f x ge0 pl0 c0 t0 =
+  print_info ("explore_term: " ^ term_construct t0);
   print_dbg dbg ("[> explore_term: " ^ term_construct t0 ^ ":\n" ^ term_to_string t0);
   let tv0 = inspect t0 in
   let x0, flag = f x ge0 pl0 c0 tv0 in
@@ -778,8 +903,11 @@ let rec explore_term dbg dfs #a f x ge0 pl0 c0 t0 =
         explore_term dbg dfs f x1 ge0 pl1 None hd
       else x1, convert_ctrl_flag flag1
     | Tv_Abs br body ->
+      print_info ("starting genv_push_binder");
       let ge1 = genv_push_binder ge0 br false None in
+      print_info ("starting abs_update_opt_typ_or_comp");
       let c1 = abs_update_opt_typ_or_comp br c0 ge1.env in
+      print_info ("recursion");
       explore_term dbg dfs f x0 ge1 pl1 c1 body
     | Tv_Arrow br c0 -> x0, Continue (* TODO: we might want to explore that *)
     | Tv_Type () -> x0, Continue
@@ -2153,6 +2281,9 @@ let pp_tac () : Tac unit =
 assume type meta_info
 assume val focus_on_term : meta_info
 
+let end_proof () =
+  tadmit_t (`())
+
 let unsquash_equality (t:term) : Tac (option (term & term)) =
   begin match term_as_formula t with
   | Comp (Eq _) l r -> Some (l, r)
@@ -2174,7 +2305,7 @@ let pp_explore (dbg dfs : bool)
     let ge = mk_genv e [] [] in
     print_dbg dbg ("[> About to explore term:\n" ^ term_to_string l);
     let x = explore_term dbg dfs #a f x ge [] c l in
-    trefl()
+    end_proof ()
   | _ -> mfail "pp_explore: not a squashed equality"
   end
 #pop-options
@@ -2366,17 +2497,21 @@ let analyze_effectful_term dbg with_gpre with_gpost res =
   (* TODO: use bv rather than term for ret_arg *)
   let ret_arg = opt_tapply (fun x -> pack (Tv_Var x)) ret_bv in
   let parents = List.Tot.map snd res.parents in
+  print_info "starting eterm_info_to_assertions";
   let ge2, asserts =
     eterm_info_to_assertions dbg with_gpre with_gpost ge1 studied_term is_let
                              is_assert info ret_arg opt_c parents [] in
+  print_info "finished eterm_info_to_assertions";
   (* Simplify and filter *)
   let asserts = simp_filter_assertions ge2.env simpl_norm_steps asserts in
+  print_info "filtered assertions";
   (* Introduce fresh variables for the shadowed ones and substitute *)
   let ge3, asserts = subst_shadowed_with_abs_in_assertions dbg ge2 shadowed_bv asserts in
+  print_info "introduced fresh variables";
   (* If not a let, insert all the assertions before the term *)
   let asserts =
     if is_let then asserts
-    else  mk_assertions (List.Tot.append asserts.pres asserts.posts) []
+    else mk_assertions (List.Tot.append asserts.pres asserts.posts) []
   in
   (* Print *)
   printout_success ge3 asserts
@@ -2385,10 +2520,12 @@ let analyze_effectful_term dbg with_gpre with_gpost res =
 val pp_analyze_effectful_term : bool -> bool -> bool -> unit -> Tac unit
 let pp_analyze_effectful_term dbg with_gpre with_gpost () =
   try
+    print_info "start";
     let res = find_focused_term_in_current_goal dbg in
+    print_info "found term";
     analyze_effectful_term dbg with_gpre with_gpost res;
-    trefl()
-  with | MetaAnalysis msg -> printout_failure msg; trefl()
+    end_proof ()
+  with | MetaAnalysis msg -> printout_failure msg; end_proof ()
        | err -> (* Shouldn't happen, so transmit the exception for debugging *) raise err
 
 (**** Split conjunctions in an assert *)
@@ -2454,8 +2591,8 @@ let pp_split_assert_conjs dbg () =
   try
     let res = find_focused_assert_in_current_goal dbg in
     split_assert_conjs dbg res;
-    trefl()
-  with | MetaAnalysis msg -> printout_failure msg; trefl()
+    end_proof ()
+  with | MetaAnalysis msg -> printout_failure msg; end_proof ()
        | err -> (* Shouldn't happen, so transmit the exception for debugging *) raise err
 
 (**** Term unfolding in assert *)
@@ -2846,7 +2983,7 @@ let pp_unfold_in_assert_or_assume dbg () =
   try
     let res = find_focused_assert_in_current_goal dbg in
     unfold_in_assert_or_assume dbg res;
-    trefl()
-  with | MetaAnalysis msg -> printout_failure msg; trefl()
+    end_proof ()
+  with | MetaAnalysis msg -> printout_failure msg; end_proof ()
        | err -> (* Shouldn't happen, so transmit the exception for debugging *) raise err
 
